theories/GScope.v
@@ -103,17 +103,9 @@ Proof.
   eapply typing_gscope. eassumption.
 Qed.
 
-Inductive gscope_parg Σ : parg → Prop :=
-| gscope_pvar : gscope_parg Σ pvar
-| gscope_pforce t : gscope Σ t → gscope_parg Σ (pforce t)
-| gscope_psymb x l : Forall (gscope_parg Σ) l → gscope_parg Σ (psymb x l).
-
-Definition gscope_pat Σ p :=
-  Forall (gscope_parg Σ) p.(pat_args).
-
 Definition gscope_rule Σ rule :=
   Forall (gscope Σ) rule.(cr_env) ∧
-  gscope_pat Σ rule.(cr_pat) ∧
+  gscope Σ (rule.(cr_pat) <[ rule.(cr_sub) ]) ∧
   gscope Σ rule.(cr_rep) ∧
   gscope Σ rule.(cr_typ).
 
@@ -131,53 +123,6 @@ Proof.
     + constructor. all: assumption.
 Qed.
 
-Lemma gscope_plinst_args_inv (f : parg → nat → term * nat) Σ pl l n r :
-  Forall (λ p, ∀ k t m, f p k = (t, m) → gscope Σ t → gscope_parg Σ p) pl →
-  fold_left (λ '(acc, k) p, let '(t, m) := f p k in (t :: acc, m)) pl r = (l, n) →
-  Forall (gscope Σ) l →
-  Forall (gscope Σ) (fst r) ∧ Forall (gscope_parg Σ) pl.
-Proof.
-  intros hl e h.
-  induction hl as [| p pl hp hl ih] in r, l, n, e, h |- *.
-  - cbn in e. subst. cbn. intuition constructor.
-  - cbn in e. eapply ih in e as h'. 2: assumption.
-    destruct r as [acc k]. cbn.
-    destruct f as [t m] eqn:e'. cbn in h'.
-    rewrite Forall_cons_iff in h' |- *.
-    intuition eauto.
-Qed.
-
-Lemma gscope_plinst_arg_inv Σ p k t m :
-  plinst_arg p k = (t, m) →
-  gscope Σ t →
-  gscope_parg Σ p.
-Proof.
-  intros e ht.
-  induction p using parg_ind in k, t, m, ht, e |- *.
-  - constructor.
-  - constructor. cbn in e. inversion e. assumption.
-  - cbn in e. destruct plinst_args eqn: es.
-    inversion e. subst. clear e.
-    constructor.
-    apply gscope_apps_inv in ht as [_ ht].
-    eapply Forall_rev in ht. rewrite rev_involutive in ht.
-    eapply gscope_plinst_args_inv in es. all: intuition eauto.
-Qed.
-
-Lemma gscope_plinst_inv Σ k p :
-  gscope Σ (plinst k p) →
-  gscope_pat Σ p.
-Proof.
-  intros h.
-  unfold plinst in h.
-  destruct plinst_args eqn:e.
-  apply gscope_apps_inv in h as [_ h].
-  eapply Forall_rev in h. rewrite rev_involutive in h.
-  unfold gscope_pat.
-  eapply gscope_plinst_args_inv in e. 1,3: intuition eauto.
-  rewrite Forall_forall. intros. eauto using gscope_plinst_arg_inv.
-Qed.
-
 Lemma rule_typing_gscope Σ Ξ Δ r :
   rule_typing Σ Ξ Δ r →
   gscope_rule Σ r.
@@ -185,7 +130,6 @@ Proof.
   intros (hctx & [i hty] & hl & hr).
   eapply typing_gscope in hl as gl, hr as gr, hty.
   eapply wf_gscope in hctx.
-  eapply gscope_plinst_inv in gl.
   rewrite Forall_app in hctx.
   unfold gscope_rule. intuition eauto.
 Qed.
@@ -226,27 +170,6 @@ Proof.
       revert σ hσ. fix aux2 2. intros σ hσ.
       destruct hσ as [| u σ h hσ]. 1: constructor.
       constructor. all: eauto.
-  }
-  all: match goal with h : _ |- _ => solve [ eapply h ; eauto ] end.
-Qed.
-
-Lemma gscope_parg_ind_alt :
-  ∀ (Σ : gctx) (P : parg → Prop),
-    P pvar →
-    (∀ t, gscope Σ t → P (pforce t)) →
-    (∀ x l, Forall (gscope_parg Σ) l → Forall P l → P (psymb x l)) →
-    ∀ p, gscope_parg Σ p → P p.
-Proof.
-  intros Σ P hvar hforce hsymb.
-  fix aux 2. move aux at top.
-  intros p h. destruct h as [| | x l h ].
-  3:{
-    eapply hsymb. 1: assumption.
-    revert l h.
-    fix aux1 2.
-    intros l h. destruct h as [| p l hp hl].
-    - constructor.
-    - constructor. all: eauto.
   }
   all: match goal with h : _ |- _ => solve [ eapply h ; eauto ] end.
 Qed.
