theories/Typing.v
@@ -264,18 +264,13 @@ Inductive ewf (Σ : gctx) : ectx → Prop :=
     inst_typing_ Σ Ξ (typing Σ Ξ) ∙ ξ' Ξ' →
     ewf Σ ((E, ξ') :: Ξ).
 
-(** Computation rule typing
-
-  TODO: We could also have some pattern typing to make sure forced terms are
-  indeed forced.
-
-**)
+(** Computation rule typing **)
 
 Definition rule_typing Σ Ξ Δ rule :=
   let k := length rule.(cr_env) in
   wf Σ Ξ (Δ ,,, rule.(cr_env)) ∧
   (∃ i, Σ ;; Ξ | Δ ,,, rule.(cr_env) ⊢ rule.(cr_typ) : Sort i) ∧
-  Σ ;; Ξ | Δ ,,, rule.(cr_env) ⊢ plinst k rule.(cr_pat) : rule.(cr_typ) ∧
+  Σ ;; Ξ | Δ ,,, rule.(cr_env) ⊢ rule.(cr_pat) <[ rule.(cr_sub) ] : rule.(cr_typ) ∧
   Σ ;; Ξ | Δ ,,, rule.(cr_env) ⊢ rule.(cr_rep) : rule.(cr_typ).
 
 (** Global environment typing **)
